some definitions in lambda formalisation.

coqfiles/vaje.v
@@ -1,4 +1,32 @@
-Inductive list (A : Type) : Type :=
-| Nil {_} : list
-| Cons : A -> list -> list.
-                      
+Module list_ex.
+  Inductive list (A : Type) : Type :=
+  | Nil : list A
+  | Cons : A -> list A -> list A.
+  
+  Arguments Nil {A}.
+  Arguments Cons {A} a l.
+  Variable X : Type.
+  
+  Infix "::" := Cons (at level 60, right associativity).
+  
+  Fixpoint join (A B: list X) : list X:=
+    match A with
+    | Nil => B
+    | Cons x y => x :: (join y B)
+    end.
+  
+  Notation "[ ]" := Nil.
+  Notation "[ x ; y ; .. ; z ]" := (Cons x (Cons y .. (Cons z Nil) ..)).
+  Infix "++" := join.
+  
+  Theorem join_nil (xs: list X) : xs ++ [] = xs.
+  Proof.
+    induction xs.
+    simpl.
+    tauto.
+    simpl.
+    rewrite IHxs.
+    tauto.
+  Qed.
+End list_ex.
+
