coqfiles/lambda.v
@@ -1,0 +1,45 @@
+From Coq Require Import Strings.String.
+
+Module types.
+  Inductive ty : Type :=
+  | unit_t : ty
+  | bool_t : ty
+  | arrow_t : ty -> ty -> ty.
+End types.
+
+Module terms.
+  Inductive tm : Type :=
+  | var : string -> tm
+  | unit : tm
+  | true : tm
+  | false : tm
+  | app : tm -> tm -> tm
+  | lam : string -> tm -> tm
+  | if_then_else : tm -> tm -> tm -> tm.
+  
+  Fixpoint substitute (x : string) (e v : tm) : tm :=
+    match v with
+    | var y => if (string_dec x y) then e else var y
+    | unit => unit
+    | true => true
+    | false => false
+    | app f value => app (substitute x e f) (substitute x e value)
+    | lam variable body => if string_dec x variable
+                          then lam variable body
+                          else lam variable (substitute x e body)
+    | if_then_else cond passed failed =>
+      if_then_else (substitute x e cond) (substitute x e passed) (substitute x e failed)
+    end.
+End terms.
+
+Module val.
+Inductive value : terms.tm -> Prop :=
+| unit : value terms.unit
+| true : value terms.true
+| false : value terms.false
+| lam x e : value (terms.lam x e).
+End val.
+
+Module int.
+  Inductive step : terms.tm -> terms.tm -> Prop :=
+    | app1 
